complete cleanup of memory interface vs instance and proper encapsulation

theories/memory.v
@@ -1,84 +1,81 @@
-(** a typeclass for a Wasm memory *)
-(* (C) J. Pichon - see LICENSE.txt *)
+(** a typeclass for a Wasm mem interface and specification *)
 
-Require Import BinNat.
-Require Import bytes.
-From mathcomp Require Import ssreflect ssrbool ssrfun eqtype.
-
-Module Memory.
-
-Definition mem_make_t Mem_t := byte -> N -> Mem_t.
-Definition mem_length_t Mem_t := Mem_t -> N.
-Definition mem_grow_t Mem_t := N -> Mem_t -> Mem_t.
-Definition mem_lookup_t Mem_t := N -> Mem_t -> option byte.
-Definition mem_update_t Mem_t := N -> byte -> Mem_t -> option Mem_t.
-
-Definition mem_ax_lookup_out_of_bounds
-  (Mem_t : Type)
-  (mem_make : mem_make_t Mem_t)
-  (mem_length : mem_length_t Mem_t)
-  (mem_grow : mem_grow_t Mem_t)
-  (mem_lookup : mem_lookup_t Mem_t)
-  (mem_update : mem_update_t Mem_t) :=
-  forall mem i, N.ge i (mem_length mem) -> mem_lookup i mem = None.
-
-Definition mem_ax_lookup_make
-  (Mem_t : Type)
-  (mem_make : mem_make_t Mem_t)
-  (mem_length : mem_length_t Mem_t)
-  (mem_grow : mem_grow_t Mem_t)
-  (mem_lookup : mem_lookup_t Mem_t)
-  (mem_update : mem_update_t Mem_t) :=
-  forall i len b, N.lt i len -> mem_lookup i (mem_make b len) = Some b.
-
-Definition mem_ax_lookup_update
-  (Mem_t : Type)
-  (mem_make : mem_make_t Mem_t)
-  (mem_length : mem_length_t Mem_t)
-  (mem_grow : mem_grow_t Mem_t)
-  (mem_lookup : mem_lookup_t Mem_t)
-  (mem_update : mem_update_t Mem_t) :=
-  forall mem mem' i b, N.lt i (mem_length mem) -> Some mem' = mem_update i b mem -> mem_lookup i mem' = Some b.
-
-Definition mem_ax_lookup_skip
-  (Mem_t : Type)
-  (mem_make : mem_make_t Mem_t)
-  (mem_length : mem_length_t Mem_t)
-  (mem_grow : mem_grow_t Mem_t)
-  (mem_lookup : mem_lookup_t Mem_t)
-  (mem_update : mem_update_t Mem_t) :=
-  forall mem mem' i i' b, i <> i' -> Some mem' = mem_update i' b mem -> mem_lookup i mem' = mem_lookup i mem.
-
-Definition mem_ax_length_constant_update
-  (Mem_t : Type)
-  (mem_make : mem_make_t Mem_t)
-  (mem_length : mem_length_t Mem_t)
-  (mem_grow : mem_grow_t Mem_t)
-  (mem_lookup : mem_lookup_t Mem_t)
-  (mem_update : mem_update_t Mem_t) :=
-  forall i b mem mem', Some mem' = mem_update i b mem -> mem_length mem' = mem_length mem.
-
+From Coq Require Import BinNat.
+From Wasm Require Import bytes common.
+From HB Require Import structures.
+From mathcomp Require Import ssrbool eqtype.
 
 Set Implicit Arguments.
 Unset Strict Implicit.
 Unset Printing Implicit Defensive.
 
+Section Memory.
 
-Section ClassDef.
+  Class Memory := {
+      mem_t : Type;
+      mem_make : byte -> N -> mem_t;
+      mem_length : mem_t -> N;
+      mem_lookup : N -> mem_t -> option byte;
+      mem_grow : N -> mem_t -> mem_t;
+      mem_update : N -> byte -> mem_t -> option mem_t;
 
-Record mixin_of (Mem_t : Type) : Type := Mixin {
-  mem_make : byte -> N -> Mem_t;
-  mem_length : Mem_t -> N;
-  mem_grow : mem_grow_t Mem_t;
-  mem_lookup : mem_lookup_t Mem_t;
-  mem_update : N -> byte -> Mem_t -> option Mem_t;
-  _ : mem_ax_lookup_out_of_bounds Mem_t mem_make mem_length mem_grow mem_lookup mem_update;
-  _ : mem_ax_lookup_make Mem_t mem_make mem_length mem_grow mem_lookup mem_update;
-  _ : mem_ax_lookup_update Mem_t mem_make mem_length mem_grow mem_lookup mem_update;
-  _ : mem_ax_lookup_skip Mem_t mem_make mem_length mem_grow mem_lookup mem_update;
-  _ : mem_ax_length_constant_update Mem_t mem_make mem_length mem_grow mem_lookup mem_update;
-}.
+      mem_eq_dec:
+      forall (m1 m2: mem_t),
+        {m1 = m2} + {m1 <> m2};
+      
+      mem_lookup_oob :
+      forall mem i,
+        N.ge i (mem_length mem) ->
+        mem_lookup i mem = None;
+      
+      mem_make_length :
+      forall b len,
+        mem_length (mem_make b len) = len;
 
-End ClassDef.
+      mem_make_lookup :
+      forall i len b,
+        N.lt i len ->
+        mem_lookup i (mem_make b len) = Some b;
+      
+      mem_update_exists :
+      forall mem i b,
+        N.lt i (mem_length mem) ->
+        { mem' | mem_update i b mem = Some mem'};
 
+      mem_update_lookup :
+      forall mem mem' i b,
+        mem_update i b mem = Some mem' ->
+        mem_lookup i mem' = Some b;
+      
+      mem_update_lookup_ne :
+      forall mem mem' i i' b,
+        i <> i' ->
+        mem_update i' b mem = Some mem' ->
+        mem_lookup i mem' = mem_lookup i mem;
+      
+      mem_update_length :
+      forall i b mem mem',
+        mem_update i b mem = Some mem' ->
+        mem_length mem' = mem_length mem;
+
+      mem_grow_lookup :
+      forall i n mem mem',
+        N.lt i (mem_length mem) ->
+        mem_grow n mem = mem' ->
+        mem_lookup i mem' = mem_lookup i mem;
+
+      mem_grow_length :
+      forall n mem mem',
+        mem_grow n mem = mem' ->
+        mem_length mem' = N.add (mem_length mem) n;
+    }.
+
+Context `{Memory}.
+  
+Definition mem_eqb v1 v2 : bool := mem_eq_dec v1 v2.
+Definition eqmemP : Equality.axiom mem_eqb :=
+  eq_dec_Equality_axiom mem_eq_dec.
+
+HB.instance Definition mem_eqMixin := hasDecEq.Build mem_t eqmemP.
+  
 End Memory.
