theories/typing_inversion.v
@@ -9,6 +9,8 @@ Unset Strict Implicit.
 Unset Printing Implicit Defensive.
 
 Section Typing_inversion_be.
+
+Context `{memory: Memory}.
   
 (* Some quality of life lemmas *)
 (* Upd: these lemmas are deprecated; it is encouraged to directly use subtyping rule. *)
@@ -451,7 +453,7 @@ Ltac e_typing_ind HType :=
 
 Section Typing_inversion_e.
              
-Context {hfc: host_function_class}.
+Context `{hfc: host_function_class} `{memory: Memory}.
 
 (** Typing lemmas **)
 
@@ -811,7 +813,7 @@ Ltac invert_e_typing :=
 (* Some more complicated lemmas *)
 Section Typing_inversion_e.
 
-Context `{hfc: host_function_class}.
+Context `{hfc: host_function_class} `{memory: Memory}.
   
 (* inst_typing inversion *)
 Lemma inst_t_context_local_empty: forall s i C,
